### Simple Steady State

$$
c + k = k^\alpha l^{1 - \alpha} + (1 - \delta)k \\
1 = \alpha k^{\alpha - 1} l^{1 - \alpha} + 1 - \delta \\
\frac{\psi \phi l^{\phi - 1}}{c^{-\eta}} = (1 - \alpha) k^{\alpha} l^{-\alpha}
$$

$$
\frac{k}{l} = \bigg(\frac{\delta}{\alpha}\bigg)^{\frac{1}{\alpha - 1}}
\\~\\
c = \frac{\delta}{\alpha} k - \delta k = \frac{\delta(1 - \alpha)}{\alpha} k
$$

$$
\psi\phi \cdot \frac{\big(\frac{\delta}{\alpha}\big)^{\frac{1 - \phi}{\alpha - 1}} k^{\phi - 1}}{\big(\frac{\delta(1 - \alpha)}{\alpha}\big)^{-\eta} k^{-\eta}}
$$